# Original Question

There is a spin 1/2 particle with magnetic moment mu (= gamma*Sz), aligned with a magnetic field pointing in the +Z direction. Suddenly, the magnetic field is turned off, and another one is turned on along the +Y direction; both fields have the same magnitude, B. The average of the z-component of the particle’s moment starts oscillating. What is its oscillation frequency?

---

# R1 response

The problem involves a spin-1/2 particle with magnetic moment \(\mu = \gamma S_z\) initially aligned with a magnetic field in the +Z direction. When the magnetic field is suddenly switched to the +Y direction with the same magnitude \(B\), we need to determine the oscillation frequency of the average z-component of the particle's magnetic moment.

1. **Initial Hamiltonian**: The initial Hamiltonian is \(H_{\text{initial}} = -\gamma B S_z\), and the particle is in the eigenstate \(| \uparrow_z \rangle\).

2. **Final Hamiltonian**: After the magnetic field is switched to the +Y direction, the new Hamiltonian is \(H_{\text{final}} = -\gamma B S_y\). The particle's state right after the switch remains \(| \uparrow_z \rangle\), which is not an eigenstate of \(H_{\text{final}}\).

3. **Time Evolution**: The time evolution operator is \(U(t) = \exp(-i H_{\text{final}} t / \hbar)\). For spin-1/2 systems, the eigenstates of \(S_y\) are \(| \pm y \rangle\). The initial state \(| \uparrow_z \rangle\) can be expressed as a superposition of \(| +y \rangle\) and \(| -y \rangle\).

4. **Expectation Value of \(S_z\)**:
   - The state evolves under the new Hamiltonian, leading to oscillations in the expectation value of \(S_z\).
   - The expectation value \(\langle S_z \rangle\) is calculated using the time-evolved state \(| \psi(t) \rangle = U(t) | \uparrow_z \rangle\).

5. **Key Calculations**:
   - The eigenstates of \(S_y\) are \(| \pm y \rangle = \frac{1}{\sqrt{2}}(| \uparrow_z \rangle \pm i | \downarrow_z \rangle)\).
   - The time evolution results in the state \(| \psi(t) \rangle = \cos(\theta) | \uparrow_z \rangle - \sin(\theta) | \downarrow_z \rangle\) where \(\theta = \gamma B t / 2\).
   - The expectation value \(\langle S_z \rangle = \frac{\hbar}{2} \cos(2\theta) = \frac{\hbar}{2} \cos(\gamma B t)\).

6. **Oscillation Frequency**: The argument of the cosine function \(\cos(\gamma B t)\) gives the angular frequency \(\omega = \gamma B\). Therefore, the oscillation frequency is \(\gamma B\).

The final answer is \(\boxed{\gamma B}\).

---

# R1 reasoning

Okay, let me try to figure this problem out. So, the scenario is a spin-1/2 particle with magnetic moment mu, which is equal to gamma times Sz, initially aligned with a magnetic field in the +Z direction. Then suddenly, the magnetic field is turned off and another one is turned on along the +Y direction, both with the same magnitude B. We need to find the oscillation frequency of the average z-component of the particle's moment. Hmm, alright.

First, I need to recall some Quantum Mechanics here. The magnetic moment is related to the spin, and in the presence of a magnetic field, the interaction Hamiltonian is given by H = -μ·B. Since originally the magnetic field is in the +Z direction, the initial Hamiltonian would be H_initial = -gamma * B * S_z. The particle is aligned with this field, so initially it's in the ground state of that Hamiltonian, which is the spin-up state along Z, right? So the initial state is |+Z> or |↑_z>.

Then, the magnetic field is suddenly switched to the +Y direction with the same magnitude. So the new Hamiltonian is H_final = -gamma * B * S_y. The particle's state doesn't change instantaneously when the magnetic field is switched, correct? So the state right after the magnetic field is turned to Y will still be the initial state |↑_z>, but now it's no longer an eigenstate of the new Hamiltonian, which is in terms of S_y. Therefore, the state will evolve under the new Hamiltonian, leading to some time dependence. The question is about the expectation value of S_z as a function of time, and its oscillation frequency.

So the key here is to find how the expectation value <S_z> evolves over time under the new Hamiltonian H_final, right? The oscillation frequency should be determined by the energy difference between the eigenstates of H_final, which are the eigenstates of S_y. Since the particle is initially in a state that is a superposition of these eigenstates, the time evolution will cause oscillations in <S_z>.

Let me recall that the spin operators S_x, S_y, S_z for spin-1/2 particles are proportional to the Pauli matrices. Specifically, S_i = (ħ/2) σ_i for i = x, y, z. But let's see, gamma is the gyromagnetic ratio, which relates the magnetic moment to the spin operator: mu = gamma S, so H = -mu·B. Therefore, H_initial was -gamma B S_z, and H_final is -gamma B S_y.

But we can write the time evolution under H_final using the time evolution operator U = exp(-i H_final t / ħ). Then the state at time t will be |psi(t)> = U |↑_z>. The expectation value of S_z will be <psi(t)| S_z |psi(t)>.

So perhaps I need to find this expectation value as a function of time and read off the oscillation frequency. Let's try to compute this step by step.

First, some setup. Let's define H_final = -gamma B S_y. For a spin-1/2 system, S_y is (ħ/2) σ_y. Therefore, H_final can be written as:

H_final = -gamma B ( ħ / 2 ) σ_y = - (gamma B ħ / 2 ) σ_y

Therefore, the time evolution operator will be:

U(t) = exp( -i H_final t / ħ ) = exp( i (gamma B ħ / 2 ) σ_y t / ħ ) = exp( i (gamma B / 2 ) t σ_y )

Simplifying, that's exp( i (gamma B t / 2 ) σ_y )

Since σ_y is a Pauli matrix, the exponential can be calculated using the identity exp(i θ σ_y) = I cosθ + i σ_y sinθ, where θ is gamma B t / 2. Let's confirm this identity. For any Pauli matrix, we have exp( i θ σ_i ) = I cosθ + i σ_i sinθ. So, yes, that works because the square of σ_i is the identity matrix, so the Taylor series will split into even and odd terms.

So, applying that:

U(t) = I cos( gamma B t / 2 ) + i σ_y sin( gamma B t / 2 )

Therefore, the time evolution operator expressed like this. Now, let's express the initial state |↑_z>. In the z-basis, that's the column vector (1, 0). Let me represent the spin states as two-component spinors. The eigenstates of S_z are (1,0) and (0,1). The initial state |↑_z> is (1, 0).

The state at time t is then |psi(t)> = U(t) |↑_z>. Let's compute this.

First, write out U(t) as a matrix. σ_y is:

σ_y = [ [0, -i], [i, 0] ]

So, i σ_y is [ [0, 1], [-1, 0] ]

Then, U(t) is:

cos(theta) [ [1, 0], [0, 1] ] + [ [0, 1], [-1, 0] ] sin(theta), where theta = gamma B t / 2

Therefore, U(t) becomes:

[ [cos(theta), sin(theta)],
  [-sin(theta), cos(theta)] ]

Applying this matrix to the spinor (1, 0), we get:

First component: cos(theta)*1 + sin(theta)*0 = cos(theta)

Second component: -sin(theta)*1 + cos(theta)*0 = -sin(theta)

So, |psi(t)> = [ cos(theta), -sin(theta) ]^T

Or,

|psi(t)> = cos(theta) |↑_z> - sin(theta) |↓_z>

Now, to find the expectation value of S_z at time t.

First, the operator S_z is (ħ/2) σ_z, so <S_z> = <psi(t)| S_z |psi(t)>

σ_z is the matrix [ [1, 0], [0, -1] ], so multiplying by ħ/2, S_z = (ħ/2) [ [1, 0], [0, -1] ]

Therefore, the expectation value is:

(ħ/2) [ cos(theta) conjugate, -sin(theta) conjugate ] [ [1, 0], [0, -1] ] [ cos(theta) ]
                                                                             [ -sin(theta) ]

Since the components are real (assuming everything is real?), so conjugates don't matter here.

Calculating the matrix multiplication:

First, multiply σ_z with the column vector [ cos(theta), -sin(theta) ]:

[ 1*cos(theta) + 0*(-sin(theta) ) , 0*cos(theta) + (-1)*(-sin(theta)) ] ^ T ? Wait, more carefully:

No, applying σ_z matrix to the vector [ cos(theta), -sin(theta) ] gives:

First component: 1 * cos(theta) + 0 * (-sin(theta)) = cos(theta)

Second component: 0 * cos(theta) + (-1) * (-sin(theta)) = sin(theta)

Then, left multiplying by the row vector [ cos(theta), -sin(theta) ] gives:

cos(theta)*cos(theta) + (-sin(theta))*sin(theta) = cos^2(theta) - sin^2(theta)

Therefore, the expectation value <S_z> is (ħ/2) [ cos^2(theta) - sin^2(theta) ]

But we know that cos^2(theta) - sin^2(theta) = cos(2 theta)

So, <S_z> = (ħ/2) cos(2 theta)

Recalling that theta = (gamma B t)/2, so,

Filling this in: <S_z> = (ħ/2) cos( 2 * (gamma B t)/2 ) = (ħ/2) cos( gamma B t )

Therefore, the expectation value of S_z oscillates as cos(gamma B t), with angular frequency omega = gamma B. Therefore, the frequency f is omega/(2 pi) = gamma B / (2 pi). But usually, frequency in these contexts is given as the angular frequency. Wait, the question says "oscillation frequency". Which is it asking for? It depends on the definition. In physics, angular frequency is often just called frequency when it's multiplied by time. But here, the problem probably wants angular frequency. Let me check.

The user is puzzled, defining:

"A spin 1/2 particle with magnetic moment mu (= gamma*Sz), aligned with a magnetic field pointing in the +Z direction. Suddenly, magnetic field is turned off, and another one turned on along the +Y direction; both fields same magnitude B. The average of the z-component of the particle’s moment starts oscillating. What is its oscillation frequency?"

Without further units, but assuming standard notation where gamma is the gyromagnetic ratio (which is gamma = mu / S_z, but here mu is given as gamma * S_z, so gamma would be the ratio mu/S_z ). Regardless, from the calculation, the <S_z> has angular frequency gamma B. Thus, the frequency would be omega = gamma B.

But wait, in our calculation, <S_z> is (ħ/2) cos(gamma B t). Remember, though, our initial expression had H_final being proportional to sigma_y, then we found theta= gamma B t / 2.

But let me check if there's an error in the calculation.

Wait. H_final is in terms of S_y. Let's make sure that when I derived U(t), whether it's correct.

H_final = -gamma * B * S_y.

But we had previously, using S_y = (ħ/2) sigma_y, so H = -gamma B (ħ/2) sigma_y.

So time evolution is given by U = exp( -i H t / ħ ). Which becomes:

exp( -i (-gamma B (ħ/2) sigma_y ) t / ħ ) = exp( i gamma B t (1/2) sigma_y )

So as we had, which is exp( i (gamma B t / 2 ) sigma_y ), which expanded to I cos(theta) + i sigma_y sin(theta), where theta = gamma B t /2.

Wait, but when we apply U to |↑_z>, then we obtained a resulting state [ cos(theta), -sin(theta) ].

Wait a second. Let me check:

Multiplying the matrix U(t) [ [ cos(theta), sin(theta) ], [-sin(theta), cos(theta) ] ]

with [1; 0] gives [ cos(theta); - sin(theta) ].

But why does the second component have a negative sign? Because the U(t) matrix as derived is:

cos(theta) * I + i sigma_y sin(theta) which when written out, gives [ cos(theta), sin(theta) ] in the first row ?

Wait, sigma_y is [[0, -i], [i, 0]], so i sigma_y is [[0, 1], [-1, 0]]. Therefore,

cos(theta) * [[1, 0],[0,1]] + sin(theta) * [[0,1],[-1,0]] gives:

[[cos(theta), sin(theta)], [ -sin(theta), cos(theta) ]]

Yes, that's correct. So the second component is -sin(theta). So when you multiply that matrix with |↑_z> which is [1;0], you get [ cos(theta) ; -sin(theta) ].

Therefore, the expectation value comes out to be (ħ/2) [cos^2(theta) - sin^2(theta) ] = (ħ/2) cos(2 theta).

That makes sense because cos(2 theta) is twice the angle, so the angular frequency is 2*theta/t. Since theta is gamma B t /2, so 2 theta /t = gamma B.

Therefore, omega = 2 theta/t = gamma B. Thus the angular frequency is gamma*B.

But wait, angular frequency is 2 pi times the ordinary frequency f. So depending on what the question is asking for, but strictly speaking, the oscillation frequency is gamma*B as the angular frequency. But if they want the ordinary frequency in cycles per second, then divide by 2 pi. So the answer requires gamma*B/(2 pi). But let's check.

Wait, in the time dependence, we have cos(gamma*B t), so the argument is gamma*B t, meaning the angular frequency is omega = gamma*B. Therefore, the frequency f is omega/(2 pi) = gamma B / (2 pi). However, in some contexts, especially when talking about Larmor frequency, it's common to express it as omega_L = gamma B, and the "frequency" is often given as the angular frequency. However, since the problem asks for the oscillation frequency, which in physics usually refers to angular frequency if they want an answer in terms of gamma and B without factors of 2 pi, unless specified. But maybe the Larmor frequency here.

But perhaps I need to check: in the case of spin precession, the angular frequency (Larmor frequency) is omega = gamma B, so frequency is omega / (2 pi). However, when the Hamiltonian is H = - gamma B S_y, the energy eigenvalues are E = ± (gamma B ħ / 2 ). The energy difference is Delta E = gamma B ħ.

Then, the oscillation frequency between states is Delta E / ħ = gamma B. Wait, in Rabi oscillations, when you have a superposition of energy eigenstates, the oscillation frequency is determined by the energy difference.

Yes, in general, for two energy levels E_1 and E_2, the oscillation frequency for transitions between them would be (E_2 - E_1)/ħ.

But in our case, the energy eigenvalues of H_final are E_1 = (gamma B ħ / 2 ) and E_2 = (-gamma B ħ / 2 ), so Delta E = gamma B ħ.

Therefore, the frequency (= omega) would be Delta E / ħ = gamma B. So angular frequency is gamma B, and the frequency f is gamma B / (2 pi). However, in the oscillation of expectation values, the angular frequency seen in the expectation value (in terms of the cosine term) was gamma B. Therefore, when they ask for oscillation frequency, if they mean the angular frequency (commonly denoted as omega) then the answer is gamma B. If they want cycles per second frequency, it's gamma B / (2 pi). But given that the problem states that the average starts oscillating with a given frequency, and given that the formula we derived has cos(gamma B t), so angular frequency is gamma B, I think in the context of the problem, especially if the answer is to be expressed in terms of gamma and B, we just put gamma B as the angular frequency. But perhaps the answer can depend on convention of what's considered frequency.

But let's check standard definition. The Larmor frequency is defined as omega_L = gamma B, which is the angular frequency. In MRI and other contexts, they often refer to Larmor frequency as just gamma B. So, that seems likely.

Wait. To make sure, here are a few steps again:

We have an initial state |↑_z>, which is not an eigenstate of the Hamiltonian H = - gamma B S y.

So it's a superposition of the eigenstates of S_y. The eigenstates of S_y are |+y> and |–y>, which can be written as (|↑_z> + i |↓_z>)/sqrt(2) and (|↑_z> – i |↓_z>)/sqrt(2) } and correspond to eigenvalues +ħ/2 and -ħ/2.

So, the initial state |↑_z> can be expressed in terms of |+y> and |–y> as follows:

|↑_z> = (|+y> + |–y>)/sqrt(2).

When the Hamiltonian H = - gamma B S y is turned on, each eigenstate evolves in time with a phase factor e^{-i E_i t / ħ}. Therefore,

|psi(t)> = (  |+y> e^{-i E_+ t / ħ} + |–y> e^{-i E_- t / ħ}  ) / sqrt(2)

where E_+ = - gamma B (ħ/2 ), and E_- = + gamma B (ħ/2 ). Wait, that depends on the direction. So wait.

Wait, Hamiltonian is H = - gamma B S y; the eigenvalues of S y are ħ/2 and -ħ/2, so the eigenvalues for H are E_+ = - gamma B (ħ/2 ) and E_- = + gamma B (ħ/2 ), since H = - gamma B S y. Therefore, E_+ = - (gamma B ħ / 2 ), E_- = gamma B ħ / 2.

Therefore, the time evolution would be:

|psi(t)> = [ e^{i gamma B ħ t / 2 ħ} |+y> + e^{-i gamma B ħ t / 2 ħ} |–y> ] / sqrt(2) = [ e^{i gamma B t / 2 } |+y> + e^{-i gamma B t / 2 } |–y> ] / sqrt(2)

So then, to express this in terms of |↑_z> and |↓_z>,

Recall that |+y> = (|↑> + i |↓>)/sqrt(2) and |–y> = (|↑> - i |↓>)/sqrt(2). So, plugging back in,

|psi(t)> = [ e^{i gamma B t /2 } (|↑> + i |↓> ) /sqrt(2) + e^{-i gamma B t /2 } ( |↑> - i |↓> ) / sqrt(2) ] / sqrt(2)

Simplify:

Combine the denominators: 1/sqrt(2) * 1/sqrt(2) = 1/sqrt(2)² = 1/2.

Then,

= (1/2) [ e^{i theta } (|↑> + i |↓> ) + e^{-i theta } ( |↑> - i |↓> ) ]

where theta = gamma B t / 2.

Expanding the exponentials,

= (1/2) [ (e^{i theta } + e^{-i theta }) |↑> + i (e^{i theta } - e^{-i theta }) |↓> ]

Then, using Euler's formula:

= (1/2) [ 2 cos(theta) |↑> + i (2i sin(theta) ) |↓> ] = (1/2) [ 2 cos(theta) |↑> - 2 sin(theta) |↓> ] = cos(theta) |↑> - sin(theta) |↓>

Therefore, same result as before. So |psi(t)> = cos(theta) |↑> - sin(theta) |↓>, with theta=gamma B t / 2. Thus, the expectation value <S_z> is (ħ/2)(cos²(theta) - sin²(theta)) = (ħ/2) cos(2 theta) = (ħ/2) cos( gamma B t )

Thus, the <S_z> oscillates as a function of time as cos(gamma B t), so the angular frequency is omega = gamma B. No question.

Therefore, the oscillation frequency is gamma*B. The question says "oscillation frequency", so if we are to follow strict terminology and avoid confusion, the oscillation frequency is the number of oscillations per unit time, which is omega/(2 pi) = gamma B/(2 pi). However, when we write the time dependence as cos(gamma B t), the oscillation frequency in terms of angular frequency omega=gamma B, whereas in cycles per second (Hz), it's f = gamma B/(2 pi). Therefore, to check, if the problem says "frequency", then if in particle physics it is more common to use angular frequency (I mean Physicists often use angular frequency when they say frequency unless stated. Let's remember that.)

Wait, the standard Larmor frequency is omega_L = gamma B, so here, the frequency would omega_L. For example, in Magnetic resonance, the Larmor frequency is given as gamma B_0. So another way omega = gamma B. So probably answer desired is omega = gamma B.

Alternatively, perhaps there a miscalculation here, let's think again, but just to be sure.

Looking at the expression for <S_z> as (ħ/2) cos(gamma B t ). The argument of the cosine is gamma B t, so the angular frequency is omega = gamma B. Therefore, the oscillation frequency is omega. So the answer is gamma B.

But see, taking an example, for example, a spin in a magnetic field in a different direction than the original.

Alternatively, think using the Heisenberg picture. When the field is along Y, then the Hamiltonian is H = -gamma B S y. In Heisenberg’s picture, the time evolution of S_z is governed by the equation of motion. We can calculate dS_z/dt = (1/iħ)[ S_z, H ].

Compute [ S_z, H ] = [ S_z, -gamma B S_y ] = -gamma B [ S_z, S_y ] = -gamma B (iħ S_x )

Therefore, dS_z/dt = (1/iħ)( -gamma B iħ S_x ) = -gamma B S_x.

Then, we need dS_x/dt: compute [S_x, H] = [ S_x, -gamma B S_y ] = -gamma B [ S_x, S_y ] = -gamma B ( iħ S_z ) So, dS_x/dt = (1 /iħ)( -gamma B iħ S_z ) = -gamma B S_z.

Similarly,

dS_y/dt = 0 since [ H, S_y ] = [ -gamma B S_y, S_y ] =0.

Wait, H = - gamma B S y => [S y, H ]=0. So S_y is conserved: dS_y/dt=0 However, the original state is |↑>,
So S_y expectation will remain the same? Do we need S_x and whose derivatives might oscillate.

Wait, but in our case the initial state is |↑> in z-direction, so ⟨ S_y ⟩ is 0 initially. However, let's check in the equation,

Since:

dS_z/dt = -gamma B S_x

dS_x/dt = -gamma B (- S_z )

Wait, if I made a mistake in signs.

Wait, let's do the calculation again carefully.

Given H = -gamma B S_y.

Then dS_z/dt = (1/iħ ) [ S_z, H ] = (1/iħ ) [ S_z, -gamma B S_y ].

= (- gamma B / iħ ) [ S_z, S_y ].

The commutator [ S_z, S_y ] = iħ S_x.

Thus,

= ( - gamma B / iħ ) (iħ S_x ) = - gamma B S_x.

Similarly, then dS_x/dt = [ S_x, H ] / iħ = [ S_x, -gamma B S_y ] / iħ = (- gamma B / iħ ) [ S_x, S_y ].

[ S_x, S_y ] = iħ S_z.

Thus,

= (- gamma B / iħ ) (iħ S_z ) = - gamma B S_z.

Then, so the equations are:

dS_z/dt = - gamma B S_x

dS_x/dt = - gamma B S_z

Wait, this gives:

Let me write equations.

dS_z / dt = - gamma B S_x   ---(1)

dS_x / dt = - gamma B S_z   ---(2)

Differentiating (1) with respect to time:

d²S_z/dt² = -gamma B dS_x/dt = -gamma B (-gamma B S_z ) )= gamma² B² S_z

Thus:

d²S_z/dt² + (gamma^2 B^2 ) S_z = 0

Which is the equation of a harmonic oscillator with angular frequency omega = gamma B.

Therefore, the solution is S_z (t) = A cos(gamma B t ) + B sin(gamma B t )

Assuming initial conditions at t=0, the S_z will be maximum and dS_z/dt = -gamma B S_x.

At t=0, if the state is |↑_z>, then <S_z(0)> = ħ / 2, and <S_x(0)> is zero.

Wait, but not operator values! Hmm.

Wait, in the Heisenberg picture, operators evolve, the states stay the same.

At t=0, H is turned on. The state is |↑_z>, which remains stationary in Heisenberg's picture.

Thus:

At t=0, ⟨ S_z (0) ⟩ = ⟨ ↑_z | S_z (0) | ↑_z ⟩ = ħ/2

⟨ S_x (0) ⟩ = 0.

Therefore, in the solution of S_z (t) = A cos(omega t ) + B sin(omega t ), impose

At t=0: S_z(0) = ħ/2 = A ?

But actually, since Heisenberg's equations give operators, but perhaps it's more accurate to write amplitudes. Either way, solutions S_z (t) is solution to the equation with sin and cos. But from the previous result we found S_z will oscillate with angular frequency gamma B, so this time derivative approach gives the same answer.

Therefore, confirming that the frequency should be gamma B.

Hence, the answer is simply gamma B. So the oscillation frequency, as given by the angular frequency, is gamma multiplied by B.

But perhaps the problem is picking up this specific based on time evolution of sigma_z.

Yes.

Therefore, the box around gamma B. The oscillation frequency of the average z-component is gamma*B.



**Final Answer**
The oscillation frequency is \boxed{\gamma B}.


---

